examples/pseudo_bool/pb_normaliseScript.sml
@@ -1,0 +1,389 @@
+(*
+  Normalization from pb_preconstraint into pb_constraint
+*)
+
+open preamble pb_preconstraintTheory pb_constraintTheory;
+
+val _ = new_theory "pb_normalise";
+
+val _ = numLib.prefer_num();
+
+(* Convert a list of pbc to one with ≥ constraints only *)
+Definition pbc_ge_def:
+  (pbc_ge (GreaterEqual xs n) = [GreaterEqual xs n]) ∧
+  (pbc_ge (Equal xs n) =
+    let xs' = MAP (λ(c:int,l). (-c,l)) xs in
+      [GreaterEqual xs n; GreaterEqual xs' (-n)])
+End
+
+Theorem eq_disj:
+  (∀x. x = a ∨ x = b ⇒ P x) ⇔ P a ∧ P b
+Proof
+  metis_tac[]
+QED
+
+Theorem eval_term_negate:
+  ∀ls.
+  (MAP (eval_term w) (MAP (λ(c,l). (-c,l)) ls)) =
+  (MAP (\i. -i) (MAP (eval_term w) ls))
+Proof
+  Induct>>simp[]>>
+  Cases>>rw[eval_term_def]>>
+  intLib.ARITH_TAC
+QED
+
+Theorem iSUM_negate:
+  ∀ls. iSUM (MAP (\i. -i) ls) = -iSUM ls
+Proof
+  Induct>>simp[iSUM_def]>>
+  intLib.ARITH_TAC
+QED
+
+Theorem pbc_ge_thm:
+  ∀c.
+  satisfies w (set (pbc_ge c)) ⇔
+  satisfies_pbc w c
+Proof
+  Cases>>
+  simp[pbc_ge_def,satisfies_def]>>
+  rw[EQ_IMP_THM]
+  >- (
+    fs[satisfies_pbc_def,eq_disj,eval_term_negate,iSUM_negate]>>
+    intLib.ARITH_TAC) >>
+  fs[satisfies_pbc_def,eval_term_negate,iSUM_negate]>>
+  intLib.ARITH_TAC
+QED
+
+Definition term_lt_def[simp]:
+  term_lt (_,l1) (_,l2) = (lit_var l1 < lit_var l2)
+End
+
+Definition term_le_def[simp]:
+  term_le (_,l1) (_,l2) = (lit_var l1 <= lit_var l2)
+End
+
+(* Ensure compact LHS in preconstraint form:
+  sort by variables *)
+Definition compact_lhs_def:
+  (compact_lhs ((c1:int,l1)::(c2,l2)::cs) n =
+    if lit_var l1 = lit_var l2 then
+      if l1 = l2 then
+        compact_lhs ((c1+c2,l1)::cs) n
+      else
+        compact_lhs ((c1-c2,l1)::cs) (n+c2)
+    else
+      let (cs',n') = compact_lhs ((c2,l2)::cs) n in
+      ((c1,l1)::cs',n')) ∧
+  (compact_lhs c n = (c,n))
+End
+
+Theorem compact_lhs_MEM:
+  ∀xs n xs' n' y l.
+  compact_lhs xs n = (xs',n') ∧
+  MEM (y,l) xs' ⇒
+  ∃y'. MEM (y',l) xs
+Proof
+  ho_match_mp_tac (theorem "compact_lhs_ind")>>
+  rw[compact_lhs_def]>> fs[]
+  >- metis_tac[]
+  >- metis_tac[]
+  >- (
+    pairarg_tac>>gs[]>>rw[]>>fs[]>>rw[]>>
+    metis_tac[])
+  >> metis_tac[]
+QED
+
+Theorem transitive_term_le:
+  transitive term_le
+Proof
+  simp[transitive_def]>>
+  rpt Cases >>
+  simp[term_le_def]
+QED
+
+Theorem transitive_term_lt:
+  transitive term_lt
+Proof
+  simp[transitive_def]>>
+  rpt Cases >>
+  simp[term_lt_def]
+QED
+
+Theorem lit_var_eq_term_le:
+  lit_var l1 = lit_var l2 ⇒
+  (term_le (a,l1) x ⇔ term_le (b,l2) x)
+Proof
+  Cases_on`x`>>rw[term_le_def]
+QED
+
+Theorem compact_lhs_no_dup:
+  ∀xs n xs' n'.
+  SORTED term_le xs ∧
+  compact_lhs xs n = (xs',n') ⇒
+  SORTED term_lt xs'
+Proof
+  ho_match_mp_tac (theorem "compact_lhs_ind")>>
+  rw[compact_lhs_def]>> fs[]
+  >- (
+    first_x_assum match_mp_tac>>
+    qpat_x_assum `SORTED _ _` mp_tac>>
+    DEP_REWRITE_TAC[SORTED_EQ]>>simp[transitive_term_le]>>
+    metis_tac[lit_var_eq_term_le])
+  >- (
+    first_x_assum match_mp_tac>>
+    qpat_x_assum `SORTED _ _` mp_tac>>
+    DEP_REWRITE_TAC[SORTED_EQ]>>simp[transitive_term_le]>>
+    metis_tac[lit_var_eq_term_le])>>
+  pairarg_tac>>fs[]>>rw[]>>
+  qpat_x_assum `SORTED _ _` mp_tac>>
+  DEP_REWRITE_TAC[SORTED_EQ]>>
+  simp[transitive_term_le,transitive_term_lt]>>
+  simp[FORALL_PROD]>>rw[]>>
+  drule compact_lhs_MEM>>
+  disch_then drule>>strip_tac>>
+  fs[]>>first_x_assum drule>>
+  fs[]
+QED
+
+Theorem iSUM_PERM:
+  ∀l1 l2. PERM l1 l2 ⇒
+  iSUM l1 = iSUM l2
+Proof
+  ho_match_mp_tac PERM_IND>>rw[iSUM_def]>>
+  intLib.ARITH_TAC
+QED
+
+Theorem iSUM_QSORT_term_le[simp]:
+  iSUM (MAP (eval_term w) (QSORT $≤ l)) =
+  iSUM (MAP (eval_term w) l)
+Proof
+  match_mp_tac iSUM_PERM>>
+  match_mp_tac PERM_MAP>>
+  metis_tac[QSORT_PERM,PERM_SYM]
+QED
+
+Theorem eval_lit_eq_flip:
+  q * eval_lit w r = q + (-q * eval_lit w (negate r))
+Proof
+  Cases_on`r` \\ EVAL_TAC
+  \\ Cases_on`w a` \\ EVAL_TAC
+  \\ fs[]
+QED
+
+Theorem compact_lhs_sound:
+  ∀xs n xs' n'.
+  compact_lhs xs n = (xs',n') ⇒
+  iSUM (MAP (pb_preconstraint$eval_term w) xs) + n = iSUM (MAP (pb_preconstraint$eval_term w) xs') + n'
+Proof
+  ho_match_mp_tac (theorem "compact_lhs_ind")>>
+  rw[compact_lhs_def]>> fs[]
+  >- (
+    (* l1 = l2 *)
+    fs[iSUM_def]>>
+    intLib.ARITH_TAC)
+  >- (
+    (* l1 = negate l2 *)
+    fs[iSUM_def]>>
+    qmatch_goalsub_abbrev_tac` A + _ + _`>>
+    REWRITE_TAC[Once eval_lit_eq_flip]>>
+    `negate l2 = l1` by
+      (Cases_on`l1`>>Cases_on`l2`>>fs[])>>
+    fs[Abbr`A`]>>
+    qpat_x_assum`_ = _ + _` sym_sub_tac>>
+    simp[integerTheory.INT_SUB_RDISTRIB]>>
+    qmatch_goalsub_abbrev_tac`_ * wl2 + _ +_ = _ - _ + is + _`>>
+    rpt (pop_assum kall_tac)>>
+    intLib.ARITH_TAC)>>
+  pairarg_tac>>fs[]>>
+  rw[]>>
+  fs[iSUM_def]>>
+  intLib.ARITH_TAC
+QED
+
+Definition mk_coeff_def:
+  (mk_coeff c (Pos v) = c) ∧
+  (mk_coeff c (Neg v) = -c:int)
+End
+
+Definition normalize_lhs_def:
+  (normalize_lhs [] acc n = (REVERSE acc,n)) ∧
+  (normalize_lhs ((x,l)::xs) acc n =
+    let v = lit_var l in
+    if x < 0 then
+      normalize_lhs xs ((mk_coeff x l,v)::acc) (n+x)
+    else if x > 0 then normalize_lhs xs ((mk_coeff x l,v)::acc) n
+    else normalize_lhs xs acc n)
+End
+
+Theorem normalize_lhs_normalizes:
+  ∀ls acc n ls' n'.
+  normalize_lhs ls acc n = (ls',n') ⇒
+  iSUM (MAP (pb_preconstraint$eval_term w) ls) + &(SUM (MAP (eval_term w) acc)) + n =
+  &(SUM (MAP (eval_term w) ls')) + n'
+Proof
+  Induct>>rw[normalize_lhs_def,iSUM_def]
+  >-
+    metis_tac[SUM_REVERSE,MAP_REVERSE] >>
+  Cases_on`h`>>fs[normalize_lhs_def]>>
+  every_case_tac>>fs[]
+  >- intLib.ARITH_TAC>>
+  first_x_assum drule>>
+  simp[GSYM integerTheory.INT_ADD]
+  >- (
+    qmatch_goalsub_abbrev_tac`&SUM _ + qq`>>
+    `qq = q * eval_lit w r` by
+      (fs[Abbr`qq`]>>Cases_on`r`>>simp[mk_coeff_def]>>
+      rename1`b2n( w a)`>>
+      Cases_on`w a`>>simp[]>>
+      intLib.COOPER_TAC)>>
+    rw[] >>
+    rename1`A +B + C + D = E`>>
+    pop_assum mp_tac>> rpt (pop_assum kall_tac)>> intLib.ARITH_TAC)
+  >- (
+    qmatch_goalsub_abbrev_tac`&SUM _ + qq`>>
+    `qq + q  = q * eval_lit w r` by (
+      fs[Abbr`qq`]>>Cases_on`r`>>simp[mk_coeff_def]>>
+      rename1`b2n (w a)`>>
+      Cases_on`w a`>>simp[]>>
+      intLib.ARITH_TAC)>>
+    rw[] >>
+    rename1`A +B + C + D = E`>>
+    ntac 2 (pop_assum mp_tac)>> rpt (pop_assum kall_tac)>> intLib.ARITH_TAC)
+  >- (
+    `q=0` by intLib.ARITH_TAC>>
+    simp[])
+QED
+
+Definition pbc_to_npbc_def:
+  (pbc_to_npbc (GreaterEqual lhs n) =
+    let (lhs',m') = compact_lhs (QSORT term_le lhs) 0 in
+    let (lhs'',m'') = normalize_lhs lhs' [] 0 in
+    let rhs = if n-(m'+m'') ≥ 0 then Num(n-(m'+m'')) else 0 in
+    PBC lhs'' rhs) ∧
+  (pbc_to_npbc (Equal xs n) = PBC [] 0)
+End
+
+Definition normalize_def:
+  normalize pbf =
+  let pbf' = FLAT (MAP pbc_ge pbf) in
+  MAP pbc_to_npbc pbf'
+End
+
+Theorem pbc_to_npbc_thm:
+  (∀xs n. pbc ≠ Equal xs n) ⇒
+  (satisfies_pbc w pbc ⇔ satisfies_npbc w (pbc_to_npbc pbc))
+Proof
+  Cases_on`pbc`>>fs[]>>
+  rw[satisfies_pbc_def,satisfies_npbc_def,pbc_to_npbc_def]>>
+  pairarg_tac>>fs[]>>
+  pairarg_tac>>fs[]>>
+  drule compact_lhs_sound>>
+  disch_then(qspec_then`w` assume_tac)>>fs[]>>
+  drule normalize_lhs_normalizes>>
+  disch_then(qspec_then`w` assume_tac)>>fs[]>>
+  simp[satisfies_npbc_def]>>
+  intLib.ARITH_TAC
+QED
+
+Theorem normalize_thm:
+  satisfies w (set pbf) ⇔
+  satisfies w (set (normalize pbf))
+Proof
+  simp[normalize_def]>>
+  qmatch_goalsub_abbrev_tac`MAP _ pbf'`>>
+  `satisfies w (set pbf) ⇔ satisfies w (set pbf')` by
+    (simp[Abbr`pbf'`]>>
+    Induct_on`pbf`>>
+    simp[]>>
+    metis_tac[pbc_ge_thm])>>
+  simp[]>>
+  `!x. MEM x pbf' ⇒ (∀xs n. x ≠ Equal xs n)` by
+    (simp[Abbr`pbf'`,MEM_FLAT,MEM_MAP,PULL_EXISTS]>>
+    Cases_on`y`>>simp[pbc_ge_def]>>
+    rw[]>>simp[])>>
+  pop_assum mp_tac>>
+  rpt(pop_assum kall_tac)>>
+  Induct_on`pbf'`>>simp[]>>
+  rw[]>>
+  metis_tac[pbc_to_npbc_thm]
+QED
+
+Theorem lit_var_negate[simp]:
+  lit_var (negate r) = lit_var r
+Proof
+  Cases_on`r`>>simp[]
+QED
+
+Theorem normalize_lhs_compact1:
+  ∀lhs acc n lhs' n'.
+  normalize_lhs lhs acc n = (lhs',n') ∧
+  SORTED $< (MAP SND (REVERSE acc) ++ MAP (lit_var o SND) lhs) ⇒
+  SORTED $< (MAP SND lhs')
+Proof
+  Induct>>simp[normalize_lhs_def]>>
+  Cases>>simp[normalize_lhs_def]>>rw[]>>
+  first_x_assum match_mp_tac>>
+  asm_exists_tac>>fs[]
+  >- (
+    PURE_REWRITE_TAC[Once (GSYM APPEND_ASSOC),APPEND]>>
+    fs[])
+  >- (
+    PURE_REWRITE_TAC[Once (GSYM APPEND_ASSOC),APPEND]>>
+    fs[]) >>
+  pop_assum mp_tac>>
+  DEP_REWRITE_TAC[SORTED_APPEND,SORTED_EQ]  >>
+  CONJ_TAC>- simp[transitive_def]>>
+  simp[]
+QED
+
+Theorem normalize_lhs_compact2:
+  ∀lhs acc n lhs' n'.
+  normalize_lhs lhs acc n = (lhs',n') ∧
+  EVERY (λc. c ≠ 0) (MAP FST acc) ⇒
+  EVERY (λc. c ≠ 0) (MAP FST lhs')
+Proof
+  Induct>>simp[normalize_lhs_def]
+  >-
+    simp[EVERY_MAP]>>
+  Cases>>fs[normalize_lhs_def]>>rw[]>>
+  first_x_assum match_mp_tac>>
+  asm_exists_tac>>fs[]>>
+  Cases_on`r`>>fs[mk_coeff_def]>>
+  intLib.ARITH_TAC
+QED
+
+Theorem compact_pbc_to_npbc:
+  compact (pbc_to_npbc c)
+Proof
+  Cases_on`c`>>rw[pbc_to_npbc_def]>>
+  pairarg_tac>>fs[]>>
+  pairarg_tac>>fs[]>>
+  imp_res_tac compact_lhs_no_dup>>
+  pop_assum mp_tac>>
+  impl_tac>- (
+    match_mp_tac QSORT_SORTED>>
+    fs[transitive_term_le]>>
+    simp[total_def]>>
+    Cases>>Cases>>simp[])>>
+  strip_tac>>
+  CONJ_TAC>- (
+    match_mp_tac normalize_lhs_compact1>>
+    asm_exists_tac>>
+    simp[sorted_map]>>
+    qmatch_goalsub_abbrev_tac`_ tlt _`>>
+    `tlt = term_lt` by
+      simp[Abbr`tlt`,FUN_EQ_THM,FORALL_PROD]>>
+    fs[])>>
+  match_mp_tac normalize_lhs_compact2>>
+  asm_exists_tac>>
+  simp[]
+QED
+
+Theorem normalize_compact:
+  EVERY compact (normalize pbf)
+Proof
+  simp[normalize_def,EVERY_MAP,compact_pbc_to_npbc]
+QED
+
+val _ = export_theory();
+
