examples/pseudo_bool/pb_parseScript.sml
@@ -1,0 +1,29 @@
+(*
+  Parse and print for pb_preconstraint, pb_check
+*)
+
+open preamble pb_preconstraintTheory pb_normaliseTheory pb_checkTheory;
+
+val _ = new_theory "pb_parse";
+
+val _ = numLib.prefer_num();
+
+(* printing of string pbc *)
+Definition lit_string_def:
+  (lit_string (Pos v) = v) ∧
+  (lit_string (Neg v) = strlit "~" ^ v)
+End
+
+Definition lhs_string_def:
+  lhs_string xs =
+  concatWith (strlit" ") (MAP(λ(c,l). concat [int_to_string #"-" c; strlit " " ; lit_string l]) xs)
+End
+
+Definition pbc_string_def:
+  (pbc_string (Equal xs i) = concat [lhs_string xs; strlit " = "; int_to_string #"-" i]) ∧
+  (pbc_string (GreaterEqual xs i) = concat [lhs_string xs; strlit " >= "; int_to_string #"-" i])
+End
+
+
+val _ = export_theory();
+
