examples/pseudo_bool/README.md
@@ -15,5 +15,11 @@ Pseudo-boolean constraints proof format and checker
 [pb_constraintScript.sml](pb_constraintScript.sml):
 Formalisation of normalised pseudo-boolean constraints
 
+[pb_normaliseScript.sml](pb_normaliseScript.sml):
+Normalization from pb_preconstraint into pb_constraint
+
+[pb_parseScript.sml](pb_parseScript.sml):
+Parse and print for pb_preconstraint, pb_check
+
 [pb_preconstraintScript.sml](pb_preconstraintScript.sml):
 Formalisation of (un-normalised) pseudo-boolean constraints with 'a var type
